ratchet/Denote/Ext.lean
@@ -342,8 +342,9 @@ theorem Ext.isExactInst_mono {m m₂ : Machine} (he : Ext m m₂) {v : Value} {n
     cases v with
     | ref o =>
       simp only [Bool.and_eq_true, decide_eq_true_eq, beq_iff_eq] at h ⊢
-      obtain ⟨hlt, hco⟩ := h
-      exact ⟨Nat.lt_of_lt_of_le hlt he.size, by rw [realClassOf, he.get o hlt]; exact hco⟩
+      obtain ⟨⟨hlt, heig⟩, hco⟩ := h
+      exact ⟨⟨Nat.lt_of_lt_of_le hlt he.size, by rw [he.get o hlt]; exact heig⟩,
+        by rw [he.get o hlt]; exact hco⟩
     | _ => simp_all
 
 theorem Ext.isAName_mono {m m₂ : Machine} (he : Ext m m₂) {v : Value} {n : String}
